\section{Cauchy's integral formula}
\lecture{6}{29/1}

\begin{proposition}
    If $\gamma: [a,b] \to \C$ is a contour and 
    $\{f_n\}_{n = 1}^\infty$
    is a sequence of continuous functions 
    $f_n: \gamma([a,b]) \to \C$
    converging uniformly on $\gamma([a,b])$
    to a continuous function 
    $f: \gamma([a,b]) \to \C$
    then
    \[
        \lim_{n \to \infty} \int_\gamma f_n(z) \,dz
        = \int_\gamma f(z) \,dz.
    \]
\end{proposition}

\begin{proof}
    The proof to this comes from the analogous fact
    from Analysis I.
\end{proof}

\begin{theorem}[Cauchy's integral formula]
    Let $r > 0$, $a \in \C$, $f: B_r(a) \to \C$ be holomorphic.
    Let $\rho \in (0, r)$, then for all $w$ such that
    $\lvert w - a \rvert < \rho$ (that is, $w \in B_\rho(a)$) then
    \[ 
        f(w) = \frac1{2\pi i} 
        \int_{\lvert z - a \rvert = \rho} \frac{f(z)}{z - w} \,dz.
    \]
\end{theorem}

This is quite peculiar; it tells us that holomorphic functions are
\emph{defined} by a boundary.

\begin{proof}
    We define
    \[
        g(z) =
        \begin{cases}
            \frac{f(z) - f(w)}{z - w} & z \neq w \\
            f'(w) & z = w.
        \end{cases}
    \]
    $g$ is holomorphic away from $w$ and
    \[
        \lim_{z \to w} \frac{f(z) - f(w)}{z - w} = f'(w)
    \]
    and so $g$ is continuous at $w$ and thus $g$ is continuous.
    Note that $B_r(a)$ is starlike.
    Hence, we have met the requirements fore Cauchy's theorem for
    starlike domains and thus
    \begin{align*}
        \int_{\lvert z - a \rvert = \rho} g(z) \,dz &= 0 \\
        \int_{\lvert z - a \rvert = \rho}
            \frac{f(z) - f(w)}{z - w} \,dz &= 0 \\
        \int_{\lvert z - a \rvert = \rho} \frac{f(z)}{z - w} \,dz
        &= \int_{\lvert z - a \rvert = \rho} \frac{f(w)}{z - w} \,dz.
    \end{align*}
    For $\lvert z - a \rvert = \rho$
    \begin{align*}
        \frac1{z - w} 
        &= \frac1{(z-a)\left(1 - \frac{w-a}{z-a}\right)} \\
        &= \frac1{z-a} \sum_{n=0}^\infty 
        \left(
            \frac{w-a}{z-a}
        \right)^n \\
        &= \sum_{n = 0}^\infty \frac{(w - a)^n}{(z - a)^{n + 1}}
    \end{align*}
    which is valid as 
    $\left\lvert \frac{w-a}{z-a} \right\rvert 
    = \frac{\lvert w - a \rvert}{\rho} < \frac{\rho}{\rho} = 1$.
    So
    \begin{align*}
        \int_{\lvert z - a \rvert = \rho} \frac{f(z)}{z - w} \,dz
        &= \int_{\lvert z - a \rvert = \rho} \frac{f(w)}{z - w} \,dz \\
        &= \int_{\lvert z - a \rvert = \rho} f(w) 
        \left(
            \sum_{n = 0}^\infty \frac{(w - a)^n}{(z - a)^{n + 1}}
        \right)
        \,dz.
    \end{align*}
    $\sum_{n = 0}^\infty \frac{(w - a)^n}{(z - a)^{n + 1}}$ converges
    uniformly on $\lvert z - a \rvert = \rho$ by the $M$-test.
    Hence, by the previous proposition
    \begin{align*}
        \int_{\lvert z - a \rvert = \rho} \frac{f(z)}{z - w} \,dz
        &= f(w) \sum_{n = 0}^\infty 
            \int_{\lvert z - a \rvert = \rho} 
            \frac{(w - a)^n}{(z - a)^{n + 1}}
            \,dz \\
        &= f(w) \sum_{n = 0}^\infty (w - a)^n 
            \int_{\lvert z - a \rvert = \rho}
            \frac1{(z-a)^{n+1}} \,dz.
    \end{align*}
    We have seen before that
    \[
        \int_{\lvert z \rvert = 1} \frac{1}{z^{n+1}} \,dz =
        \begin{cases}
            2\pi i & n = 0 \\
            0 & n \neq 0.
        \end{cases}
    \]
    The same result holds for any other ball.
    Hence
    \[
        \int_{\lvert z - a \rvert = \rho} \frac{f(z)}{z - w} \,dz = f(w) \cdot 2\pi i.
    \]
\end{proof}

\chapter{Features of holomorphic functions}
\section{The Cauchy-Taylor theorem and integral formula for derivatives}

Recall that power series can be differentiated in their radius of convergence;
that is, they give holomorphic functions there.
In fact, all holomorphic functions are given locally by a power series.

\begin{theorem}[Cauchy-Taylor theorem]
    Let $r > 0$, $a \in \C$, and $f: B_r(a) \to \C$ be holomorphic.
    Then $f$ has a convergent power series expansion; that is,
    \[
        f(z) = \sum^{\infty}_{n = 0} c_n (z - a)^n \tag{$\dagger$}
    \]
    for all $z \in B_r(z)$ where
    \[
        c_n = \frac{1}{2\pi i}    
        \int_{\lvert z - a \rvert = \rho}
        \frac{f(z)}{(z - a)^{n + 1}} \,dz
    \]
    for any $\rho \in (0,r)$.
\end{theorem}

We call $(\dagger)$ the taylor series of $f$ at $a$.

\begin{proof}
    For any $0 < \rho < r$ we have
    \[
        f(w) = \frac{1}{2\pi i} \int_{\lvert z - a \rvert = \rho}
        \frac{f(z)}{z - w} \,dz
    \]
    for all $w \in B_{\rho}(a)$
    by Cauchy's integral formula.
    By the geometric series formula we get
    \[
        f(w) = \frac{1}{2\pi i} \int_{\lvert z - a \rvert = \rho}
        f(w) \sum^{\infty}_{n = 0} \frac{(w - a)^n}{(z - a)^{n + 1}} \,dz 
    \]
    so the previous proof (for uniform convergence) and the previous
    proposition tells us
    \[
        f(w) = \frac{1}{2\pi i} \sum^{\infty}_{n = 0} (w - a)^n
        \int_{\lvert z - a \rvert = \rho} \frac{f(z)}{(z - a)^{n + 1}} \,dz
        = \sum^{\infty}_{n = 0} c_n (w-a)^n.
    \]
    Therefore, $f$ has a power series expansion of $B_{\rho}(a)$ so
    \[
        c_n = f^{(n)}(a) \cdot \frac1{n!}
    \]
    which does not depend on $\rho$.
    Now, as for all $w \in B_r(a): w \in B_{\rho}(a)$ for some $\rho < r$
    and hence holds for $B_r(a)$.
\end{proof}
